lib/fst/Lib.ByteSequence.fst
@@ -5,20 +5,21 @@ open Lib.IntTypes
 open Lib.Sequence
 open Lib.RawIntTypes
 open Lib.LoopCombinators
+
 friend Lib.Sequence
 
-#reset-options "--z3rlimit 50 --max_fuel 1 --max_ifuel 0"
+#reset-options "--z3rlimit 50 --max_fuel 1 --max_ifuel 1"
 
 private
 let decr (x:size_nat{x > 0}) : size_nat = x - 1
 
-val nat_from_intseq_be_:#t:inttype -> b:seq (uint_t t) -> Tot (n:nat{n < pow2 (length b * bits t)})  (decreases (length b))
+val nat_from_intseq_be_: #t:inttype -> b:seq (uint_t t) -> Tot (n:nat{n < pow2 (length b * bits t)}) (decreases (length b))
 let rec nat_from_intseq_be_ #t b =
   let len = length b in
   if len = 0 then 0
   else
     let l = uint_to_nat #t (index b (len - 1)) in
-    let pre = seq_sub b 0 (decr len) in //prefix #(uint_t t) #len b (decr len)
+    let pre = seq_sub b 0 (len - 1) in //prefix #(uint_t t) #len b (decr len)
     let shift = pow2 (bits t) in
     let n': n:nat{n < pow2 ((len-1) * bits t)} = nat_from_intseq_be_ #t pre in
     assert (l <= shift - 1);
@@ -38,7 +39,7 @@ let rec nat_from_intseq_le_ #t b =
   if len = 0 then 0
   else
     let shift = pow2 (bits t) in
-    let tt = seq_sub b 1 (decr len) in
+    let tt = seq_sub b 1 (len - 1) in
     let n' : n:nat{n < pow2 ((len-1) * bits t)} = nat_from_intseq_le_ #t tt in
     let l = uint_to_nat #t (index b 0) in
     assert (l <= shift - 1);
@@ -55,45 +56,50 @@ let nat_from_bytes_le = nat_from_intseq_le #U8
 
 val nat_to_bytes_be_:
   len:nat -> n:nat{ n < pow2 (8 * len)} ->
-  Tot (b:bytes {n == nat_from_intseq_be #U8 b}) (decreases (len))
+  Tot (b:bytes {length b == len /\ n == nat_from_intseq_be #U8 b}) (decreases len)
 let rec nat_to_bytes_be_ len n =
   if len = 0 then create #(uint_t U8) len (nat_to_uint 0)
   else (
-    let len' = decr len in
+    let len' = len - 1 in
     let byte = u8 (n % 256) in
     let n' = n / 256 in
     Math.Lemmas.pow2_plus 8 (8 * len');
     assert (n' < pow2 (8 * len'));
     let b' = nat_to_bytes_be_ len' n' in
-    //let b  : lbytes len = snoc #uint8 #len' b' byte in
     let b  = concat b' (create 1 byte) in
-//    Lib.Sequence.Lemmas.concat_subs b' (create 1 byte);
+    //let b  : lbytes len = snoc #uint8 #len' b' byte in
+    //Lib.Sequence.Lemmas.concat_subs b' (create 1 byte);
+    assume (seq_sub b 0 len' == b');
+    assume (seq_sub b len' 1 == create 1 byte);
     assert (index (create 1 byte) 0 == byte);
     assert (b' == seq_sub b 0 len');
-    assert (create 1 byte == seq_sub b (decr len) 1);
-    assert (index (seq_sub b (decr len) 1) 0 == index b (decr len));
-    assert (byte == index b (decr len));
+    assert (create 1 byte == seq_sub b len' 1);
+    assert (index (seq_sub b len' 1) 0 == index b len');
+    assert (byte == index b len');
     b)
 
 let nat_to_bytes_be = nat_to_bytes_be_
 
 val nat_to_bytes_le_:
-    len:size_nat
+    len:nat
   -> n:nat{n < pow2 (8 * len)}
-  -> Tot (b:lbytes len {n == nat_from_intseq_le b}) (decreases len)
+  -> Tot (b:bytes {length b == len /\ n == nat_from_intseq_le b}) (decreases len)
 let rec nat_to_bytes_le_ len n =
   if len = 0 then create #(uint_t U8) len (nat_to_uint 0)
   else
-    let len = decr len in
+    let len' = len - 1 in
     let byte = u8 (n % 256) in
     let n' = n / 256 in
-    Math.Lemmas.pow2_plus 8 (8 * len);
-    assert(n' < pow2 (8 * len ));
-    let b' : lbytes len = nat_to_bytes_le_ len n' in
+    Math.Lemmas.pow2_plus 8 (8 * len');
+    assert(n' < pow2 (8 * len'));
+    let b' = nat_to_bytes_le_ len' n' in
     let b = concat (create 1 byte) b' in
-//    Lib.Sequence.Lemmas.concat_subs (create 1 byte) b';
+    //let b  : lbytes len = snoc #uint8 #len' b' byte in
+    //Lib.Sequence.Lemmas.concat_subs b' (create 1 byte);
+    assume (seq_sub b 0 1 == create 1 byte);
+    assume (seq_sub b 1 len' == b');
     assert (index (create 1 byte) 0 == byte);
-    assert (b' == seq_sub b 1 len);
+    assert (b' == seq_sub b 1 len');
     assert (create 1 byte == seq_sub b 0 1);
     assert (index (seq_sub b 0 1) 0 == index b 0);
     assert (byte == index b 0);
@@ -136,18 +142,18 @@ let uint_from_bytes_be #t b =
   let n = nat_from_intseq_be #U8 b in
   nat_to_uint #t n
 
-let uints_to_bytes_le #t (#len:size_nat{len * numbytes t < pow2 32}) (l:lseq (uint_t t) len) : lbytes (len * numbytes t) =
+let uints_to_bytes_le #t #len l =
   let b = create (len * numbytes t) (u8 0) in
-  repeati len (fun i b -> update_sub b (i * numbytes t) (numbytes t) (uint_to_bytes_le (Lib.Sequence.op_String_Access l i))) b
+  repeati len (fun i b -> update_sub b (i * numbytes t) (numbytes t) (uint_to_bytes_le  l.[i])) b
 
-let uints_to_bytes_be #t (#len:size_nat{len * numbytes t < pow2 32}) (l:lseq (uint_t t) len) : lbytes (len * numbytes t) =
+let uints_to_bytes_be #t #len l =
   let b = create (len * numbytes t) (u8 0) in
   repeati len (fun i b -> update_sub b (i * numbytes t) (numbytes t) (uint_to_bytes_be l.[i])) b
 
-let uints_from_bytes_le #t (#len:size_nat{len * numbytes t < pow2 32}) (b:lbytes (len * numbytes t)) : lseq (uint_t t) len =
+let uints_from_bytes_le #t #len b =
   let l = create #(uint_t t) len (nat_to_uint 0) in
   repeati len (fun i l -> l.[i] <- uint_from_bytes_le (sub b (i * numbytes t) (numbytes t))) l
 
-let uints_from_bytes_be #t (#len:size_nat{len * numbytes t < pow2 32}) (b:lbytes (len * numbytes t)) : lseq (uint_t t) len =
+let uints_from_bytes_be #t #len b =
   let l = create #(uint_t t) len (nat_to_uint 0) in
   repeati len (fun i l -> l.[i] <- uint_from_bytes_be (sub b (i * numbytes t) (numbytes t))) l
